Encoding

Logic/Propositional/Intuitionistic/Formula.lean
@@ -148,70 +148,60 @@ end Decidable
 
 section Encodable
 
-open Nat
+abbrev Node (α) := α ⊕ Unit ⊕ Fin 3
+
+@[reducible]
+def Edge (α) : Node α → Type
+  | (Sum.inl _)                => Empty
+  | (Sum.inr $ Sum.inl _)      => Empty
+  | (Sum.inr $ Sum.inr ⟨_, _⟩) => Bool
+
+def toW : Formula α → WType (Edge α)
+  | atom a  => ⟨Sum.inl a, Empty.elim⟩
+  | falsum  => ⟨Sum.inr $ Sum.inl (), Empty.elim⟩
+  | imp p q => ⟨Sum.inr $ Sum.inr ⟨0, (by trivial)⟩, Bool.rec p.toW q.toW⟩
+  | or p q  => ⟨Sum.inr $ Sum.inr ⟨1, (by trivial)⟩, Bool.rec p.toW q.toW⟩
+  | and p q => ⟨Sum.inr $ Sum.inr ⟨2, (by trivial)⟩, Bool.rec p.toW q.toW⟩
+
+def ofW : WType (Edge α) → Formula α
+  | ⟨Sum.inl a, _⟩                => atom a
+  | ⟨Sum.inr $ Sum.inl (), _⟩     => falsum
+  | ⟨Sum.inr $ Sum.inr ⟨0, _⟩, p⟩ => imp (ofW $ p false) (ofW $ p true)
+  | ⟨Sum.inr $ Sum.inr ⟨1, _⟩, p⟩ => or (ofW $ p false) (ofW $ p true)
+  | ⟨Sum.inr $ Sum.inr ⟨2, _⟩, p⟩ => and (ofW $ p false) (ofW $ p true)
+
+lemma toW_ofW : ∀ (w : WType (Edge α)), toW (ofW w) = w
+  | ⟨Sum.inl a, _⟩                => by simp [ofW, toW, Empty.eq_elim];
+  | ⟨Sum.inr $ Sum.inl (), _⟩     => by simp [ofW, toW, Empty.eq_elim];
+  | ⟨Sum.inr $ Sum.inr ⟨0, _⟩, w⟩ => by
+    simp [ofW, toW, toW_ofW (w false), toW_ofW (w true)];
+    ext b; cases b <;> simp;
+  | ⟨Sum.inr $ Sum.inr ⟨1, _⟩, w⟩ => by
+    simp [ofW, toW, toW_ofW (w false), toW_ofW (w true)];
+    ext b; cases b <;> simp;
+  | ⟨Sum.inr $ Sum.inr ⟨2, _⟩, w⟩ => by
+    simp [ofW, toW, toW_ofW (w false), toW_ofW (w true)];
+    ext b; cases b <;> simp;
+
+def equivW (α) : Formula α ≃ WType (Edge α) where
+  toFun := toW
+  invFun := ofW
+  right_inv := toW_ofW
+  left_inv := λ p => by induction p <;> simp_all [toW, ofW]
+
+instance : (a : Node α) → Fintype (Edge α a)
+  | (Sum.inl _)           => Fintype.ofIsEmpty
+  | (Sum.inr $ Sum.inl _) => Fintype.ofIsEmpty
+  | (Sum.inr $ Sum.inr _) => Bool.fintype
+
+instance : (a : Node α) → Primcodable (Edge α a)
+  | (Sum.inl _)           => Primcodable.empty
+  | (Sum.inr $ Sum.inl _) => Primcodable.empty
+  | (Sum.inr $ Sum.inr _) => Primcodable.bool
 
 variable [Encodable α]
 
-private def encode : Formula α → Nat
-  | ⊥      => pair 0 0
-  | atom a => pair 0 ((Encodable.encode a) + 1)
-  | p ⟶ q  => pair 1 (pair (p.encode) (q.encode))
-  | p ⋏ q  => pair 2 (pair (p.encode) (q.encode))
-  | p ⋎ q  => pair 3 (pair (p.encode) (q.encode))
-
-private lemma _root_.Nat.unpair_left_lt (h : unpair e = (m, n)) (hm : 1 ≤ m) : n < e := by
-  have := Nat.pair_unpair' h;
-  induction n with
-  | zero => simp_all [pair]; aesop;
-  | succ n ih =>
-    simp_all [pair];
-    split at this;
-    . rw [←this];
-      have : 1 < succ n := LE.le.trans_lt hm (by simpa)
-      have h₁ : succ n < (succ n * succ n) := Nat.lt_mul_self_iff.mpr this;
-      have h₂ : (succ n * succ n) ≤ (succ n * succ n) + m := by apply Nat.le_add_right;
-      exact LT.lt.trans_le h₁ h₂;
-    . aesop;
-
-private def decode (e : ℕ) : Option (Formula α) :=
-  match h : e.unpair with
-  | (0, 0) => some ⊥
-  | (0, k + 1) =>
-    match Encodable.decode k with
-    | some a => some (atom a)
-    | none   => none
-  | (1, k) =>
-    match decode k.unpair.1, decode k.unpair.2 with
-    | some p, some q => some (p ⟶ q)
-    | _, _ => none
-  | (2, k) =>
-    match decode k.unpair.1, decode k.unpair.2 with
-    | some p, some q => some (p ⋏ q)
-    | _, _ => none
-  | (3, k) =>
-    match decode k.unpair.1, decode k.unpair.2 with
-    | some p, some q => some (p ⋎ q)
-    | _, _ => none
-  | _ => none
-decreasing_by
-  all_goals simp_wf;
-  . exact LE.le.trans_lt (Nat.unpair_left_le k) (Nat.unpair_left_lt h (by trivial));
-  . exact LE.le.trans_lt (Nat.unpair_right_le k) (Nat.unpair_left_lt h (by trivial));
-  . exact LE.le.trans_lt (Nat.unpair_left_le k) (Nat.unpair_left_lt h (by trivial));
-  . exact LE.le.trans_lt (Nat.unpair_right_le k) (Nat.unpair_left_lt h (by trivial));
-  . exact LE.le.trans_lt (Nat.unpair_left_le k) (Nat.unpair_left_lt h (by trivial));
-  . exact LE.le.trans_lt (Nat.unpair_right_le k) (Nat.unpair_left_lt h (by trivial));
-
-instance : Encodable (Formula α) where
-  encode := encode
-  decode := decode
-  encodek p := by
-    induction p using rec' with
-    | hfalsum => sorry;
-    | hatom a => sorry;
-    | himp p q  => sorry;
-    | hand p q  => sorry;
-    | hor p q  => sorry;
+instance : Encodable (Formula α) := Encodable.ofEquiv (WType (Edge α)) (equivW α)
 
 end Encodable
 
